reals/faster/ARbigD.v
@@ -95,12 +95,12 @@ Qed.
 Lemma bigD_div_correct (x y : bigD) (k : Z) : Qball (2 ^ k) ('app_div x y k) ('x / 'y).
 Proof.
   assert (∀ xm xe ym ye : Z, 
-      ('xm * 2 ^ xe : Q) / ('ym * 2 ^ ye : Q) = ('xm * 2 ^ (-(k - 1) + xe - ye)) / 'ym * 2 ^ (k - 1)) as E1.
+      (('xm * 2 ^ xe)%mc : Q) / (('ym * 2 ^ ye)%mc : Q) = ('xm * 2 ^ (-(k - 1) + xe - ye)) / 'ym * 2 ^ (k - 1)) as E1.
    intros.
    rewrite 2!int_pow_exp_plus by solve_propholds.
    rewrite dec_fields.dec_recip_distr.
    rewrite 2!int_pow_negate.
-   transitivity ('xm / 'ym * 2 ^ xe / 2 ^ ye * (2 ^ (k - 1) / 2 ^ (k - 1)) : Q); [| ring].
+   transitivity (('xm / 'ym * 2 ^ xe / 2 ^ ye * (2 ^ (k - 1) / 2 ^ (k - 1)))%mc : Q); [| ring].
    rewrite dec_recip_inverse by solve_propholds. ring.
   assert (∀ xm xe ym ye : Z, 
       'Z.div (Z.shiftl xm (-(k - 1) + xe - ye)) ym * 2 ^ (k - 1) - 2 ^ k  ≤ ('xm * 2 ^ xe) / ('ym * 2 ^ ye : Q)) as Pleft.
@@ -114,7 +114,7 @@ Proof.
    apply (order_preserving (.* _)).
    apply rings.flip_le_minus_l. 
    apply semirings.plus_le_compat_r; [easy |].
-   transitivity ('Z.shiftl xm (-(k - 1) + xe - ye) / 'ym - 1 : Q).
+   transitivity (('Z.shiftl xm (-(k - 1) + xe - ye) / 'ym - 1)%mc : Q).
     apply (order_preserving (+ -1)). now apply Qdiv_bounded_Zdiv.
    destruct (orders.le_or_lt 0 ym) as [E | E].
     apply rings.flip_le_minus_l. 
@@ -123,7 +123,7 @@ Proof.
      apply dec_fields.nonneg_dec_recip_compat.
      now apply semirings.preserves_nonneg.
     now apply Qpow_bounded_Zshiftl.
-   transitivity (('Z.shiftl xm (-(k - 1) + xe - ye) + 1) / 'ym : Q).
+   transitivity ((('Z.shiftl xm (-(k - 1) + xe - ye) + 1) / 'ym)%mc : Q).
     rewrite rings.plus_mult_distr_r.
     apply semirings.plus_le_compat; [reflexivity |].
     rewrite rings.mult_1_l.
@@ -150,7 +150,7 @@ Proof.
     ring_simplify. apply sm_proper. now apply commutativity.
    intros. rewrite E1, E2.
    apply (order_preserving (.* _)).
-   transitivity ('Z.shiftl xm (-(k - 1) + xe - ye) / 'ym + 1 : Q).
+   transitivity (('Z.shiftl xm (-(k - 1) + xe - ye) / 'ym + 1)%mc : Q).
     2: now apply (order_preserving (+1)); apply orders.lt_le, Qdiv_bounded_Zdiv.
    destruct (orders.le_or_lt ym 0) as [E3 | E3].
     apply semirings.plus_le_compat_r; [easy |].
@@ -158,8 +158,8 @@ Proof.
      apply dec_fields.nonpos_dec_recip_compat.
      now apply semirings.preserves_nonpos.
     now apply Qpow_bounded_Zshiftl.
-   transitivity (('Z.shiftl xm (-(k - 1) + xe - ye) + 1) / ' ym : Q).
-    apply (maps.order_preserving_flip_nonneg (.*.) (/ 'ym : Q)).
+   transitivity ((('Z.shiftl xm (-(k - 1) + xe - ye) + 1) / ' ym)%mc : Q).
+    apply (maps.order_preserving_flip_nonneg (.*.) ((/ 'ym)%mc : Q)).
      apply dec_fields.nonneg_dec_recip_compat.
      apply semirings.preserves_nonneg.
      now apply orders.lt_le.
@@ -187,7 +187,7 @@ Instance bigD_approx : AppApprox bigD := λ x k,
 Lemma bigD_approx_correct (x : bigD) (k : Z) : Qball (2 ^ k) ('app_approx x k) ('x).
 Proof.
   setoid_replace (app_approx x k) with (app_div x 1 k).
-   setoid_replace ('x : Q) with ('x / '1 : Q).
+   setoid_replace ('x : Q) with (('x / '1)%mc : Q).
     now apply bigD_div_correct.
    rewrite rings.preserves_1, dec_fields.dec_recip_1.
    now rewrite rings.mult_1_r.
